ChoiceLogic/theories/LogicQualifier.v
@@ -13,12 +13,12 @@ Section LogicQualifier.
 
 Context {V : Type} `{ValueSig V}.
 
-Local Notation bnamingT := (gmap nat atom) (only parsing).
+Local Notation BStoreT := (gmap nat V) (only parsing).
 Local Notation StoreT := (gmap atom V) (only parsing).
 Local Notation WfWorldT := (WfWorld (V := V)) (only parsing).
 
 Inductive logic_qualifier : Type :=
-  | lqual (B : gset nat) (d : aset) (prop : bnamingT → StoreT → WfWorldT → Prop).
+  | lqual (B : gset nat) (d : aset) (prop : BStoreT → StoreT → WfWorldT → Prop).
 
 Definition lqual_dom (q : logic_qualifier) : aset :=
   match q with
@@ -30,9 +30,18 @@ Definition lqual_bvars (q : logic_qualifier) : gset nat :=
   | lqual B _ _ => B
   end.
 
-Definition lqual_prop (q : logic_qualifier) : bnamingT → StoreT → WfWorldT → Prop :=
+Definition lqual_prop (q : logic_qualifier) : BStoreT → StoreT → WfWorldT → Prop :=
   match q with
   | lqual _ _ p => p
+  end.
+
+Definition lqual_open (k : nat) (x : atom) (q : logic_qualifier) : logic_qualifier :=
+  match q with
+  | lqual B d p =>
+      if decide (k ∈ B) then
+        lqual (B ∖ {[k]}) ({[x]} ∪ d)
+          (λ β σ w, ∃ v, σ !! x = Some v ∧ p (<[k := v]> β) σ w)
+      else q
   end.
 
 #[global] Instance stale_logic_qualifier : Stale logic_qualifier := lqual_dom.
@@ -40,10 +49,11 @@ Arguments stale_logic_qualifier /.
 
 Definition logic_qualifier_denote
     (q : logic_qualifier)
+    (bmap : BStoreT)
     (σ : StoreT)
     (w : WfWorldT) : Prop :=
   match q with
-  | lqual _ d p => p ∅ (store_restrict σ d) (res_restrict w d)
+  | lqual B d p => p (map_restrict V bmap B) (store_restrict σ d) (res_restrict w d)
   end.
 
 End LogicQualifier.
